thys/Pi_Calculus/Pi_cong.thy
@@ -2,14 +2,14 @@ theory Pi_cong
   imports Commitment
 begin
 
-abbreviation Tsupp :: "trm \<Rightarrow> trm \<Rightarrow> var set" where
+abbreviation Tsupp :: "proc \<Rightarrow> proc \<Rightarrow> var set" where
   "Tsupp e1 e2 \<equiv> FFVars e1 \<union> FFVars e2"
 
-lemma fresh: "\<exists>xx. xx \<notin> Tsupp (t :: trm) t2"
-  by (metis (no_types, lifting) exists_var finite_iff_le_card_var term.Un_bound term.set_bd_UNIV)
+lemma fresh: "\<exists>xx. xx \<notin> Tsupp (t :: proc) t2"
+  by (metis (no_types, lifting) exists_var finite_iff_le_card_var Proc.Un_bound Proc.set_bd_UNIV)
 
 (* Structural congurence *)
-binder_inductive cong :: "trm \<Rightarrow> trm \<Rightarrow> bool" (infix "(\<equiv>\<^sub>\<pi>)" 40) where
+binder_inductive cong :: "proc \<Rightarrow> proc \<Rightarrow> bool" (infix "(\<equiv>\<^sub>\<pi>)" 40) where
   "P = Q \<Longrightarrow> P \<equiv>\<^sub>\<pi> Q"
 | "Par P Q \<equiv>\<^sub>\<pi> Par Q P"
 | "Par (Par P Q) R \<equiv>\<^sub>\<pi> Par P (Par Q R)"
@@ -21,7 +21,7 @@ binder_inductive cong :: "trm \<Rightarrow> trm \<Rightarrow> bool" (infix "(\<e
   subgoal for R B \<sigma> x1 x2
     apply simp
     by (elim disj_forward case_prodE)
-      (auto simp: isPerm_def term.rrename_comps
+      (auto simp: isPerm_def Proc.rrename_comps
         | ((rule exI[of _ "\<sigma> _"] exI)+, (rule conjI)?, rule refl)
         | ((rule exI[of _ "\<sigma> _"])+; auto))+
   subgoal premises prems for R B x1 x2
@@ -40,7 +40,7 @@ thm cong.strong_induct
 thm cong.equiv
 
 lemma finite_Tsupp: "finite (Tsupp x1 x2)"
-  by (metis FFVars_commit_simps(5) finite_FFVars_commit finite_Un)
+  by (metis FFVars_Com_simps(5) finite_FFVars_Com finite_Un)
 
 lemma exists_fresh:
   "\<exists> z. z \<notin> set xs \<and> (z \<notin> Tsupp x1 x2)"
@@ -50,11 +50,11 @@ proof-
     using finite_Tsupp by blast
   then obtain x where "x \<notin> set xs \<union> Tsupp x1 x2"
     by (meson ex_new_if_finite finite_iff_le_card_var
-        infinite_iff_natLeq_ordLeq var_term_pre_class.large)
+        infinite_iff_natLeq_ordLeq var_Proc_pre_class.large)
   thus ?thesis by auto
 qed
 
-binder_inductive trans :: "trm \<Rightarrow> trm \<Rightarrow> bool" (infix "(\<rightarrow>)" 30) where
+binder_inductive trans :: "proc \<Rightarrow> proc \<Rightarrow> bool" (infix "(\<rightarrow>)" 30) where
   "Par (Out x z P) (Inp x y Q) \<rightarrow> Par P (usub Q z y)"
 | "P \<rightarrow> Q \<Longrightarrow> Par P R \<rightarrow> Par P Q"
 | "P \<rightarrow> Q \<Longrightarrow> Res x P \<rightarrow> Res x Q"
@@ -62,15 +62,15 @@ binder_inductive trans :: "trm \<Rightarrow> trm \<Rightarrow> bool" (infix "(\<
   subgoal for R B \<sigma> x1 x2
     apply simp
     apply (elim disj_forward exE)
-       apply  (auto simp: isPerm_def term.rrename_comps
+       apply  (auto simp: isPerm_def Proc.rrename_comps
         | ((rule exI[of _ "\<sigma> _"] exI)+, (rule conjI)?, rule refl)
         | ((rule exI[of _ "\<sigma> _"])+; auto))+
-    by (metis cong.equiv bij_imp_inv' term.rrename_bijs term.rrename_inv_simps)
+    by (metis cong.equiv bij_imp_inv' Proc.rrename_bijs Proc.rrename_inv_simps)
   subgoal for R B x1 x2
     unfolding ex_push_inwards conj_disj_distribL ex_disj_distrib ex_simps(1,2)[symmetric]
       ex_comm[where P = P for P :: "_ set \<Rightarrow> _ \<Rightarrow> _"]
     apply (elim disj_forward exE; simp; clarsimp)
-      apply (auto simp only: fst_conv snd_conv term.set)
+      apply (auto simp only: fst_conv snd_conv Proc.set)
     subgoal for x z P y Q
       apply (rule exE[OF exists_fresh[of "[x, y, z]" P Q]])
       subgoal for w
